more cleanup to SetoidRewrite
- adding a lemma about typeof_expr and exprD ensuring
  the same type
- slight generalization of setoid_rewrite with a wrapper
  function to build a simpler interface.

src/Ext/SetoidRewrite.v
@@ -1,4 +1,6 @@
 Require Import Relations.
+Require Import ExtLib.Data.Pair.
+Require Import ExtLib.Recur.GenRec.
 Require Import ExtLib.Recur.Relation.
 Require Import ExtLib.Tactics.
 Require Import MirrorCore.SymI.
@@ -51,19 +53,17 @@ Section setoid.
       | Rpointwise t r => PRpointwise t (R_to_PR r)
     end.
 
-  (** The output relation will be an instantiation of R **)
-  Variable properAt : expr sym -> PR -> option R.
-
   (** The input relation must not have variables in it? **)
   Variable atomic : tenv typ -> forall e : expr sym,
-                      (forall e', TransitiveClosure.rightTrans (@expr_acc sym) e' e -> tenv typ -> PR -> option (T * R))
-                      -> tenv typ -> R -> T.
+    (forall e', TransitiveClosure.rightTrans (@expr_acc sym) e' e -> tenv typ -> PR -> option (T * R))
+    -> tenv typ -> PR -> option (T * R).
 
   (** ?? **)
   Variable app : tenv typ -> tenv typ -> T -> T -> R -> R -> T.
   Variable abs : tenv typ -> tenv typ -> typ -> T -> R -> T.
 
-  Definition setoid_rewrite' (tus : tenv typ) : expr sym -> tenv typ -> PR -> option (T * R) :=
+  Definition setoid_rewrite' (tus : tenv typ)
+  : expr sym -> tenv typ -> PR -> option (T * R) :=
     @Fix (expr sym) _ (wf_rightTrans (@wf_expr_acc sym))
          (fun _ => tenv typ -> PR -> option (T * R))
          (fun e =>
@@ -71,76 +71,63 @@ Section setoid.
                return (forall e', TransitiveClosure.rightTrans (@expr_acc sym) e' e -> tenv typ -> PR -> option (T * R)) -> tenv typ -> PR -> option (T * R)
             with
               | App l r => fun recur tvs rel =>
+                             (** TODO: It shouldn't be necessary to type check here **)
                 match typeof_expr tus tvs r with
                   | None => None
                   | Some ty =>
                     match recur l (TransitiveClosure.RTFin _ _ _ (acc_App_l _ _)) tvs (PRfunctorial (PRguess ty) rel) with
                       | None =>
-                        match properAt (App l r) rel with
-                          | None => None
-                          | Some rel' =>
-                            Some (@atomic tus (App l r) recur tvs rel', rel')
-                        end
+                        @atomic tus (App l r) recur tvs rel
                       | Some (l', relx) =>
                         match relx with
                           | Rfunctorial rel' out =>
                             match recur r (TransitiveClosure.RTFin _ _ _ (acc_App_r _ _)) tvs
                                         (R_to_PR rel')
                             with
-                              | None => None
+                              | None =>
+                                @atomic tus (App l r) recur tvs rel
                               | Some (r', out_r) => (** maybe this is strange **)
                                 (** out_r = rel' **)
-                                Some (app tus tvs l' r' out_r out, out)
+                                Some (app tus tvs l' r' rel' out, out)
                             end
                           | _ => None (** Never happens **)
                         end
                     end
                 end
               | Abs t e' => fun recur tvs prel =>
-                              match prel with
-                                | PRpointwise t' r' =>
-                                  match recur e' (TransitiveClosure.RTFin _ _ _ (acc_Abs _ _))
-                                              (t :: tvs) r'
-                                  with
-                                    | Some (result, r'') =>
-                                      Some (abs tus tvs t result r'', Rpointwise t' r'')
-                                    | _ =>
-                                      match properAt (Abs t e') prel with
-                                        | None => None
-                                        | Some rel' =>
-                                          Some (@atomic tus (Abs t e') recur tvs rel', rel')
-                                      end
-                                  end
-                                | _ =>
-                                  match properAt (Abs t e') prel with
-                                    | None => None
-                                    | Some rel' =>
-                                      Some (@atomic tus (Abs t e') recur tvs rel', rel')
-                                  end
-                              end
+                match prel with
+                  | PRpointwise t' r' =>
+                    match recur e'
+                                (TransitiveClosure.RTFin _ _ _ (acc_Abs _ _))
+                                (t :: tvs) r'
+                    with
+                      | Some (result, r'') =>
+                        Some (abs tus tvs t result r'', Rpointwise t' r'')
+                      | _ =>
+                        @atomic tus (Abs t e') recur tvs prel
+                    end
+                  | _ =>
+                    @atomic tus (Abs t e') recur tvs prel
+                end
               | e' => fun recur tvs rel =>
-                        match properAt e' rel with
-                          | None => None
-                          | Some rel' =>
-                            Some (@atomic tus e' recur tvs rel', rel')
-                        end
+                @atomic tus e' recur tvs rel
             end).
 
   Variable typeForRbase : Rbase -> typ.
-
-  Fixpoint typeForPR (r : PR) : typ :=
-    match r with
-      | PRinj r => typeForRbase r
-      | PRguess t => t
-      | PRfunctorial l r => tyArr (typeForPR l) (typeForPR r)
-      | PRpointwise t r => tyArr t (typeForPR r)
-    end.
 
   Fixpoint typeForR (r : R) : typ :=
     match r with
       | Rinj r => typeForRbase r
       | Rfunctorial l r => tyArr (typeForR l) (typeForR r)
       | Rpointwise t r => tyArr t (typeForR r)
+    end.
+
+  Fixpoint typeForPR (r : PR) : typ :=
+    match r with
+      | PRinj r => typeForRbase r
+      | PRfunctorial l r => tyArr (typeForPR l) (typeForPR r)
+      | PRpointwise t r => tyArr t (typeForPR r)
+      | PRguess t => t
     end.
 
   Inductive instantiates : R -> PR -> Prop :=
@@ -154,24 +141,34 @@ Section setoid.
                  instantiates a b ->
                  instantiates (Rpointwise t a) (PRpointwise t b).
 
-  Variable TR : env (typD ts) -> env (typD ts) -> forall r : R, T -> typD ts nil (typeForR r) -> Prop.
+  Variable TR : env (typD ts) -> env (typD ts) ->
+                forall r : R, T -> typD ts nil (typeForR r) -> Prop.
 
   Hypothesis Hatomic
-  : forall e r r',
-      properAt e r = Some r' ->
+  : forall tus tvs e r r' result
+           (recur : forall e', TransitiveClosure.rightTrans (@expr_acc sym) e' e
+                               -> tenv typ -> PR -> option (T * R)),
+      @atomic tus e recur tvs r = Some (result, r') ->
+      (forall tvs e' r r' result pf,
+         recur e' pf tvs r = Some (result, r') ->
+         instantiates r' r /\
+         forall us vs x,
+           WellTyped_env tus us ->
+           WellTyped_env tvs vs ->
+           exprD us vs e' (typeForR r') = Some x ->
+           TR us vs r' result x) ->
       instantiates r' r /\
-      forall us vs x result (recur : forall e', TransitiveClosure.rightTrans (@expr_acc sym) e' e -> tenv typ -> PR -> option (T * R)),
-        (forall tus e' tvs r r' result pf,
-           recur e' pf tvs r = Some (result, r') ->
-           instantiates r' r /\
-           forall us vs x,
-             WellTyped_env tus us ->
-             WellTyped_env tvs vs ->
-             exprD us vs e' (typeForR r') = Some x ->
-             TR us vs r' result x) ->
-        @atomic (typeof_env us) e recur (typeof_env vs) r' = result ->
+      forall us vs x,
+        WellTyped_env tus us ->
+        WellTyped_env tvs vs ->
         exprD us vs e (typeForR r') = Some x ->
         TR us vs r' result x.
+
+  Hypothesis atomic_ext
+  : forall a b c x f g,
+      (forall e pf p q,
+         f e pf p q = g e pf p q) ->
+      @atomic a x f b c = @atomic a x g b c.
 
   Hypothesis Happ
   : forall us vs t1 t2 r1 r2 v1 v2 f,
@@ -181,7 +178,7 @@ Section setoid.
       @TR us vs t2 (app (typeof_env us) (typeof_env vs) r1 r2 t1 t2) (v1 v2).
 
   Hypothesis Habs
-  : forall us vs (t1 : typ) (t2 : R) (r1 : T) (v1 : typD ts nil t1 -> typD ts nil (typeForR t2)) f,
+  : forall us vs t1 t2 r1 v1 f,
       exprD us vs f (typeForR (Rpointwise t1 t2)) = Some v1 ->
       (forall x : typD ts nil t1, @TR us (existT _ _ x :: vs) t2 r1 (v1 x)) ->
       @TR us vs (Rpointwise t1 t2) (abs (typeof_env us) (typeof_env vs) t1 r1 t2) v1.
@@ -191,23 +188,20 @@ Section setoid.
     match e with
       | App l r =>
         match typeof_expr tus tvs r with
-          | None => None
+          | None => None (** Never happens **)
           | Some ty =>
             match setoid_rewrite' tus l tvs (PRfunctorial (PRguess ty) rel) with
               | None =>
-                match properAt (App l r) rel with
-                  | None => None
-                  | Some rel' =>
-                    Some (@atomic tus (App l r) (fun e _ => setoid_rewrite' tus e) tvs rel', rel')
-                end
+                @atomic tus (App l r) (fun e _ => setoid_rewrite' tus e) tvs rel
               | Some (l', relx) =>
                 match relx with
                   | Rfunctorial rel' out =>
                     match setoid_rewrite' tus r tvs (R_to_PR rel') with
-                      | None => None
+                      | None =>
+                        @atomic tus (App l r) (fun e _ => setoid_rewrite' tus e) tvs rel
                       | Some (r', out_r) => (** maybe this is strange **)
                         (** out_r = rel' **)
-                        Some (app tus tvs l' r' out_r out, out)
+                        Some (app tus tvs l' r' rel' out, out)
                     end
                   | _ => None (** Never happens **)
                 end
@@ -220,36 +214,36 @@ Section setoid.
               | Some (result, r'') =>
                 Some (abs tus tvs t result r'', Rpointwise t' r'')
               | _ =>
-                match properAt (Abs t e') rel with
-                  | None => None
-                  | Some rel' =>
-                    Some (@atomic tus (Abs t e') (fun e _ => setoid_rewrite' tus e) tvs rel', rel')
-                end
+                @atomic tus (Abs t e') (fun e _ => setoid_rewrite' tus e) tvs rel
             end
           | _ =>
-            match properAt (Abs t e') rel with
-              | None => None
-              | Some rel' =>
-                Some (@atomic tus (Abs t e') (fun e _ => setoid_rewrite' tus e) tvs rel', rel')
-            end
+            @atomic tus (Abs t e') (fun e _ => setoid_rewrite' tus e) tvs rel
         end
       | e' =>
-        match properAt e' rel with
-          | None => None
-          | Some rel' =>
-            Some (@atomic tus e' (fun e _ => setoid_rewrite' tus e) tvs rel', rel')
-        end
+        @atomic tus e' (fun e _ => setoid_rewrite' tus e) tvs rel
     end.
   Proof.
     unfold setoid_rewrite'.
-    intros. erewrite Fix_eq.
-    { destruct e; reflexivity. }
-    { intros. destruct x; simpl; try reflexivity.
-      admit.
-      admit.
-      admit.
-      admit.
-      admit. }
+    intros.
+    match goal with
+      | |- context [ @Fix _ _ _ _ ?F _ ] =>
+        remember F ;
+        generalize (@Fix_equiv _ (TransitiveClosure.rightTrans (expr_acc (func:=sym))) (wf_rightTrans (wf_expr_acc (func:=sym)))
+                               _ o
+                   (fun x f g => forall a b, f a b = g a b))
+    end.
+    intro X. rewrite X; clear X.
+    { subst. destruct e; try reflexivity. }
+    { destruct x; subst; simpl; intros; eauto using atomic_ext.
+      { forward. rewrite H.
+        destruct (g x1
+                    (TransitiveClosure.RTFin (expr_acc (func:=sym)) x1
+                                             (App x1 x2) (acc_App_l x1 x2)) a (PRfunctorial (PRguess t) b)).
+        { destruct p. forward. rewrite H.
+          forward. eauto using atomic_ext. }
+        eauto using atomic_ext. }
+      destruct b; eauto using atomic_ext.
+      rewrite H. forward; eauto using atomic_ext. }
   Qed.
 
   Lemma instantiates_typeof : forall r1 r2,
@@ -260,8 +254,8 @@ Section setoid.
   Qed.
 
   Lemma inv_instantiates_functorial : forall a b c d,
-                                        instantiates (Rfunctorial a b) (PRfunctorial c d) ->
-                                        instantiates a c /\ instantiates b d.
+    instantiates (Rfunctorial a b) (PRfunctorial c d) ->
+    instantiates a c /\ instantiates b d.
   Proof.
     clear. inversion 1; subst; eauto.
   Qed.
@@ -283,8 +277,8 @@ Section setoid.
     inversion H; subst; try congruence.
   Qed.
 
-  Lemma setoid_rewrite_sound_lem
-  : forall tus e tvs r r' result,
+  Lemma setoid_rewrite'_sound_lem
+  : forall e tus tvs r r' result,
       setoid_rewrite' tus e tvs r = Some (result, r') ->
       instantiates r' r /\
       forall us vs x,
@@ -293,48 +287,45 @@ Section setoid.
         exprD us vs e (typeForR r') = Some x ->
         TR us vs r' result x.
   Proof.
-    induction e; simpl; intros.
-    admit.
-    admit.
-    admit.
-(*
-    { rewrite setoid_rewrite_eta in *.
-      generalize dependent (@Var sym v); intros.
-      forward. inv_all; subst.
-      inversion H0; clear H0; subst.
-      destruct (@Hatomic e r r' H).
-      auto. }
-    { admit. }
-    { rewrite setoid_rewrite_eta in H.
-      red_exprD. forward.
-      consider (setoid_rewrite (typeof_env us) e1 (typeof_env vs) (PRfunctorial (PRguess t) r)); intros.
-      { destruct p. forward; inv_all; subst. inversion H4; clear H4; subst.
-        specialize (@IHe1 _ _ _ _ H1); destruct IHe1.
-        eapply inv_instantiates_functorial in H0. intuition.
-        specialize (@IHe2 _ _ _ _ H3); destruct IHe2.
-        forward; subst. inv_all; subst.
-        generalize (@typ_cast_typ_eq _ _ _ _ _ _ H11); intros; subst.
-        rewrite typ_cast_typ_refl in H11. inv_all; subst.
-        eapply instantiates_R_to_PR in H6. subst.
-        simpl in H2.
-        cut (typeForR l = t); intros; subst.
-        { cut (t3 = typeForR l); intros; subst.
-          { specialize (H2 _ H9).
-            specialize (H7 _ H10).
-            eapply Happ; eauto. }
-          { revert H. revert H10. clear. admit. } }
-        { 
-          eauto using instantiates_guess. } }
-      { admit. } }
-*)
-    { rewrite setoid_rewrite'_eta in H.
-      destruct r. admit. admit. admit.
-      consider (setoid_rewrite' tus e (t :: tvs) r).
-      { destruct p; intros. inv_all; subst.
-        inversion H0; clear H0; subst.
-        specialize (IHe _ _ _ _ H). intuition.
+    refine (@expr_strong_ind _ _ _).
+    destruct e; simpl; intros; rewrite setoid_rewrite'_eta in H0;
+    eauto using Hatomic with typeclass_instances.
+    { forward.
+      consider (setoid_rewrite' tus e1 tvs (PRfunctorial (PRguess t) r)); intros;
+      eauto using Hatomic with typeclass_instances.
+      { destruct p. forward. subst.
+        consider (setoid_rewrite' tus e2 tvs (R_to_PR l));
+          eauto using Hatomic with typeclass_instances; intros.
+        destruct p. inv_all; subst.
+        generalize (H _ _ _ _ _ _ _ H2); clear H2.
+        generalize (H _ _ _ _ _ _ _ H1); clear H H1.
+        intros. destruct H; destruct H1.
+        eapply instantiates_R_to_PR in H. subst.
+        eapply inv_instantiates_functorial in H1.
+        destruct H1. split; auto.
+        intros.
+        red_exprD.
+        forward; inv_all; subst.
+        clear Habs Hatomic.
+        inversion H; clear H; subst.
+        assert (t3 = typeForR l).
+        { eapply WellTyped_env_typeof_env in H4.
+          eapply WellTyped_env_typeof_env in H5.
+          subst.
+          apply (typeof_expr_exprD_same_type _ _ _ _ _ H9 H0). }
+        subst.
+        specialize (H3 us vs _ H4 H5 H8).
+        specialize (H2 us vs _ H4 H5 H9).
+        eapply WellTyped_env_typeof_env in H4.
+        eapply WellTyped_env_typeof_env in H5. subst.
+        specialize (@Happ us vs l r' t0 t1); eauto. } }
+    { destruct r; eauto using Hatomic.
+      { consider (setoid_rewrite' tus e (t :: tvs) r); eauto using Hatomic.
+        destruct p; intros. inv_all; subst.
+        specialize (H _ _ _ _ _ _ _ H0).
+        destruct H. split.
         { constructor. auto. }
-        { clear Happ Hatomic.
+        { clear Happ Hatomic. intros.
           red_exprD. inversion x1; subst.
           revert H4. uip_all'. intros; subst.
           apply WellTyped_env_typeof_env in H2.
@@ -342,12 +333,85 @@ Section setoid.
           eapply (@Habs us vs t r0 t1 _ (Abs t e)).
           { admit. }
           { intros.
-            eapply H1; eauto. admit. admit.
-            admit. } } }
-      { admit. } }
-
-    admit.
+            eapply H1; eauto.
+            { eapply WellTyped_env_typeof_env; auto. }
+            { eapply WellTyped_env_typeof_env; auto. }
+            { generalize dependent (x2 x); intros.
+              match goal with
+                | |- ?X = Some (match ?Y with _ => _ end _) =>
+                  change Y with X ; destruct X
+              end; auto. exfalso; auto. } } } } }
   Qed.
+
+(*
+  (** TODO: I really need to work this out with [exprD'] **)
+  Lemma setoid_rewrite'_sound_lem2
+  : forall vs e tus tvs r r' result,
+      setoid_rewrite' tus e (tvs ++ typeof_env vs) r = Some (result, r') ->
+      instantiates r' r /\
+      forall us vs' x,
+        WellTyped_env tus us ->
+        WellTyped_env tvs vs ->
+        exprD' us (vs' ++ typeof_env vs) e (typeForR r') = Some x ->
+        TR us vs r' result x.
+  Proof.
+    refine (@expr_strong_ind _ _ _).
+    destruct e; simpl; intros; rewrite setoid_rewrite'_eta in H0;
+    eauto using Hatomic with typeclass_instances.
+    { forward.
+      consider (setoid_rewrite' tus e1 tvs (PRfunctorial (PRguess t) r)); intros;
+      eauto using Hatomic with typeclass_instances.
+      { destruct p. forward. subst.
+        consider (setoid_rewrite' tus e2 tvs (R_to_PR l));
+          eauto using Hatomic with typeclass_instances; intros.
+        destruct p. inv_all. inversion H3; clear H3; subst.
+        generalize (H _ _ _ _ _ _ _ H2); clear H2.
+        generalize (H _ _ _ _ _ _ _ H1); clear H H1.
+        intros. destruct H; destruct H1.
+        eapply instantiates_R_to_PR in H. subst.
+        eapply inv_instantiates_functorial in H1.
+        destruct H1. split; auto.
+        intros.
+        red_exprD.
+        forward; inv_all; subst.
+        clear Habs Hatomic.
+        inversion H; clear H; subst.
+        assert (t3 = typeForR l).
+        { eapply WellTyped_env_typeof_env in H4.
+          eapply WellTyped_env_typeof_env in H5.
+          subst.
+          apply (typeof_expr_exprD_same_type _ _ _ _ H9 H0). }
+        subst.
+        specialize (H3 us vs _ H4 H5 H8).
+        specialize (H2 us vs _ H4 H5 H9).
+        eapply WellTyped_env_typeof_env in H4.
+        eapply WellTyped_env_typeof_env in H5. subst.
+        specialize (@Happ us vs l r' t0 t1); eauto. } }
+    { destruct r; eauto using Hatomic.
+      { consider (setoid_rewrite' tus e (t :: tvs) r); eauto using Hatomic.
+        destruct p; intros. inv_all; subst.
+        inversion H1; clear H1; subst.
+        specialize (H _ _ _ _ _ _ _ H0).
+        destruct H. split.
+        { constructor. auto. }
+        { clear Happ Hatomic. intros.
+          red_exprD. inversion x1; subst.
+          revert H4. uip_all'. intros; subst.
+          apply WellTyped_env_typeof_env in H2.
+          apply WellTyped_env_typeof_env in H3. subst.
+          eapply (@Habs us vs t r0 t1 _ (Abs t e)).
+          { admit. }
+          { intros.
+            eapply H1; eauto.
+            { eapply WellTyped_env_typeof_env; auto. }
+            { eapply WellTyped_env_typeof_env; auto. }
+            { generalize dependent (x2 x); intros.
+              match goal with
+                | |- ?X = Some (match ?Y with _ => _ end _) =>
+                  change Y with X ; destruct X
+              end; auto. exfalso; auto. } } } } }
+  Qed.
+*)
 
   Definition setoid_rewrite (tus tvs : tenv typ) (e : expr sym) (r : R) : option T :=
     match setoid_rewrite' tus e tvs (R_to_PR r) with
@@ -367,7 +431,7 @@ Section setoid.
     unfold setoid_rewrite. intros.
     consider (setoid_rewrite' tus e tvs (R_to_PR r)); intros; try congruence.
     destruct p; intuition. inv_all; subst.
-    eapply setoid_rewrite_sound_lem in H. intuition.
+    eapply setoid_rewrite'_sound_lem in H. intuition.
     eapply instantiates_R_to_PR in H3. subst.
     eauto.
   Qed.
@@ -379,38 +443,49 @@ Section interface.
   Variable sym : Type. (** Symbols **)
   Variable RSym_sym : RSym (typD ts) sym.
 
+  Let tc_acc : relation (expr sym) :=
+    TransitiveClosure.rightTrans (@expr_acc sym).
+
   Record SRW_Algo (T : Type) : Type :=
   { Rbase : Type (** Relations **)
-     (** The output relation will be an instantiation of R **)
-   ; properAt : expr sym -> PR Rbase -> option (R Rbase)
-     (** The input relation must not have variables in it? **)
-   ; atomic : tenv typ -> forall e : expr sym,
-                            (forall e', TransitiveClosure.rightTrans (@expr_acc sym) e' e -> tenv typ -> (PR Rbase) -> option (T * (R Rbase)))
-                            -> tenv typ -> R Rbase -> T
-     (** ?? **)
-   ; app : tenv typ -> tenv typ -> T -> T -> R Rbase -> R Rbase -> T
-   ; abs : tenv typ -> tenv typ -> typ -> T -> R Rbase -> T
+    (** The input relation must not have variables in it? **)
+  ; atomic : tenv typ -> forall e : expr sym,
+    (forall e', tc_acc e' e -> tenv typ -> PR Rbase -> option (T * R Rbase))
+    -> tenv typ -> PR Rbase -> option (T * R Rbase)
+    (** ?? **)
+  ; app : tenv typ -> tenv typ -> T -> T -> R Rbase -> R Rbase -> T
+  ; abs : tenv typ -> tenv typ -> typ -> T -> R Rbase -> T
   }.
 
   Record SRW_AlgoOk (T : Type) (Algo : SRW_Algo T) : Type :=
   { typeForRbase : Algo.(Rbase) -> typ
   ; TR : env (typD ts) -> env (typD ts) -> forall r : R Algo.(Rbase), T -> typD ts nil (typeForR typeForRbase r) -> Prop
-  ; Hatomic
-    : forall e r r',
-      Algo.(properAt) e r = Some r' ->
-      instantiates typeForRbase r' r /\
-      forall us vs x result (recur : forall e', TransitiveClosure.rightTrans (@expr_acc sym) e' e -> tenv typ -> PR Algo.(Rbase)-> option (T * R Algo.(Rbase))),
-        (forall tus e' tvs r r' result pf,
-           recur e' pf tvs r = Some (result, r') ->
-           instantiates typeForRbase r' r /\
-           forall us vs x,
-             WellTyped_env tus us ->
-             WellTyped_env tvs vs ->
-             exprD us vs e' (typeForR typeForRbase r') = Some x ->
-             TR us vs r' result x) ->
-        @Algo.(atomic) (typeof_env us) recur (typeof_env vs) r' = result ->
-        exprD us vs e (typeForR typeForRbase r') = Some x ->
-        TR us vs r' result x
+
+  ;  Hatomic
+     : forall tus tvs e r r' result
+              (recur : forall e', tc_acc e' e
+                                  -> tenv typ -> PR Algo.(Rbase) ->
+                                  option (T * R Algo.(Rbase))),
+         Algo.(atomic) tus (e := e) recur tvs r = Some (result, r') ->
+         (forall tvs e' r r' result pf,
+            recur e' pf tvs r = Some (result, r') ->
+            instantiates typeForRbase r' r /\
+            forall us vs x,
+              WellTyped_env tus us ->
+              WellTyped_env tvs vs ->
+              exprD us vs e' (typeForR typeForRbase r') = Some x ->
+              TR us vs r' result x) ->
+         instantiates typeForRbase r' r /\
+         forall us vs x,
+           WellTyped_env tus us ->
+           WellTyped_env tvs vs ->
+           exprD us vs e (typeForR typeForRbase r') = Some x ->
+           TR us vs r' result x
+  ; atomic_ext
+    : forall a b c x f g,
+        (forall e pf p q,
+           f e pf p q = g e pf p q) ->
+        Algo.(atomic) a (e:=x) f b c = Algo.(atomic) a (e:=x) g b c
   ; Happ
     : forall us vs t1 t2 r1 r2 v1 v2 f,
         exprD us vs f (typeForR typeForRbase (Rfunctorial t1 t2)) = Some v1 ->
@@ -421,12 +496,92 @@ Section interface.
     : forall us vs t1 t2 r1 v1 f,
         exprD us vs f (typeForR typeForRbase (Rpointwise t1 t2)) = Some v1 ->
         (forall x : typD ts nil t1, @TR us (existT _ _ x :: vs) t2 r1 (v1 x)) ->
-        @TR us vs (Rpointwise t1 t2) (Algo.(abs) (typeof_env us) (typeof_env vs) t1 r1 t2) v1
+        @TR us vs (Rpointwise t1 t2)
+            (Algo.(abs) (typeof_env us) (typeof_env vs) t1 r1 t2) v1
   }.
 
-  Definition setoid_rewriteI {T} (a : SRW_Algo T) : tenv typ -> tenv typ -> expr sym -> R a.(Rbase) -> option T :=
-    @setoid_rewrite ts sym RSym_sym _ T a.(properAt) a.(atomic) a.(app) a.(abs).
+  Section from_proper.
 
+    Variable (T : Type).
+    Variable (_Rbase : Type).
+    Hypothesis (_properAt : expr sym -> PR _Rbase -> option (R _Rbase)).
+    Hypothesis (_atomic : tenv typ -> forall e : expr sym,
+                                       (forall e', tc_acc e' e -> tenv typ ->
+                                                   (PR _Rbase) -> option (T * (R _Rbase)))
+                                       -> tenv typ -> R _Rbase -> T).
+    Hypothesis (_app : tenv typ -> tenv typ -> T -> T -> R _Rbase -> R _Rbase -> T).
+    Hypothesis (_abs : tenv typ -> tenv typ -> typ -> T -> R _Rbase -> T).
+
+    Definition SRW_Algo_properAt : SRW_Algo T :=
+      {| Rbase := _Rbase
+       ; atomic := fun tus e recur tvs rel =>
+                     match _properAt e rel with
+                       | None => None
+                       | Some rel' =>
+                         Some (_atomic tus (e:=e) recur tvs rel', rel')
+                     end
+       ; app := _app
+       ; abs := _abs
+       |}.
+
+    Hypothesis typeForRbase : _Rbase -> typ.
+    Hypothesis TR : env (typD ts) -> env (typD ts) -> forall r : R _Rbase, T -> typD ts nil (typeForR typeForRbase r) -> Prop.
+    Hypothesis Hatomic
+    : forall e r r',
+        _properAt e r = Some r' ->
+        instantiates typeForRbase r' r /\
+        forall us vs x result (recur : forall e', tc_acc e' e -> tenv typ -> PR _Rbase-> option (T * R _Rbase)),
+        (forall e' tvs r r' result pf,
+           recur e' pf tvs r = Some (result, r') ->
+           instantiates typeForRbase r' r /\
+           forall vs x,
+             WellTyped_env tvs vs ->
+             exprD us vs e' (typeForR typeForRbase r') = Some x ->
+             TR us vs r' result x) ->
+        _atomic (typeof_env us) recur (typeof_env vs) r' = result ->
+        exprD us vs e (typeForR typeForRbase r') = Some x ->
+        TR us vs r' result x.
+    Hypothesis Hatomic_ext
+    : forall a b c x f g,
+        (forall e pf p q,
+           f e pf p q = g e pf p q) ->
+        _atomic a (e:=x) f b c = _atomic a (e:=x) g b c.
+    Hypothesis Happ
+    : forall us vs t1 t2 r1 r2 v1 v2 f,
+        exprD us vs f (typeForR typeForRbase (Rfunctorial t1 t2)) = Some v1 ->
+        @TR us vs (Rfunctorial t1 t2) r1 v1 ->
+        @TR us vs t1 r2 v2 ->
+        @TR us vs t2 (_app (typeof_env us) (typeof_env vs) r1 r2 t1 t2) (v1 v2).
+    Hypothesis Habs
+    : forall us vs t1 t2 r1 v1 f,
+        exprD us vs f (typeForR typeForRbase (Rpointwise t1 t2)) = Some v1 ->
+        (forall x : typD ts nil t1, @TR us (existT _ _ x :: vs) t2 r1 (v1 x)) ->
+        @TR us vs (Rpointwise t1 t2) (_abs (typeof_env us) (typeof_env vs) t1 r1 t2) v1.
+
+    Theorem SRW_AlgoOk_properAt : SRW_AlgoOk SRW_Algo_properAt.
+    Proof.
+      refine (@Build_SRW_AlgoOk _ SRW_Algo_properAt typeForRbase _ _ _ _ _);
+      simpl; eauto using Happ, Habs.
+      { intros.
+        forward; inv_all; subst.
+        destruct (@Hatomic _ _ _ H); intuition.
+        eapply H2; clear H2; eauto.
+        { instantiate (1 := recur).
+          intros.
+          specialize (@H0 _ _ _ _ _ _ H2).
+          intuition. }
+        { eapply WellTyped_env_typeof_env in H3.
+          eapply WellTyped_env_typeof_env in H4.
+          subst. reflexivity. } }
+      { intros.
+        destruct (_properAt x c); auto.
+        f_equal. f_equal. eapply Hatomic_ext. auto. }
+    Qed.
+  End from_proper.
+
+  Definition setoid_rewriteI {T} (a : SRW_Algo T)
+  : tenv typ -> tenv typ -> expr sym -> R a.(Rbase) -> option T :=
+    @setoid_rewrite ts sym RSym_sym _ T a.(atomic) a.(app) a.(abs).
 
   Theorem setoid_rewriteI_sound {T} (a : SRW_Algo T) (aC : SRW_AlgoOk a)
   : forall tus tvs e r result,
@@ -441,169 +596,5 @@ Section interface.
     destruct aC.
     eapply setoid_rewrite_sound in H; eauto.
   Qed.
+
 End interface.
-
-(**
-Section demo.
-  Variable ts : types.
-
-  Inductive sym : Type := And | Other.
-  Instance RSym_sym : RSym (typD ts) sym :=
-  { typeof_sym := fun s =>
-                    match s with
-                      | And => Some (tyArr tyProp (tyArr tyProp tyProp))
-                      | Other => Some (tyArr tyProp tyProp)
-                    end
-  ; symD := fun s =>
-              match s as s return match match s with
-                                          | And => Some (tyArr tyProp (tyArr tyProp tyProp))
-                                          | Other => Some (tyArr tyProp tyProp)
-                                        end
-                                  with
-                                    | None => unit
-                                    | Some t => typD ts nil t
-                                  end
-              with
-                | And => and
-                | Other => not
-              end
-  ; sym_eqb := fun _ _ => None
-  }.
-  Inductive Rbase := Impl | Eq.
-  Definition typeForRbase (_ : Rbase) : typ := tyProp.
-  Definition T := expr sym.
-
-  Fixpoint RD (r : R Rbase) : relation (typD ts nil (typeForR typeForRbase r)) :=
-    match r with
-      | Rfunctorial l r =>
-        (fun f g => forall x y, RD l x y -> RD r (f x) (g y))
-      | Rinj Impl => Basics.impl
-      | Rinj Eq => @eq Prop
-    end.
- Import ExtLib.Core.RelDec.
-  
-  Local Instance RelDec_Rbase : RelDec (@eq Rbase) :=
-  { rel_dec := fun a b =>
-                 match a , b with
-                   | Eq , Eq => true
-                   | Impl , Impl => true
-                   | _ , _ => false
-                 end
-  }.
-
-  Fixpoint unify (r : R Rbase) (p : PR Rbase) : bool :=
-    match p with
-      | PRguess _ => true
-      | PRinj i => match r with
-                     | Rinj i' => i ?[ eq ] i'
-                     | _ => false
-                   end
-      | PRfunctorial a b =>
-        match r with
-          | Rfunctorial a' b' => andb (unify a' a) (unify b' b)
-          | _ => false
-        end
-    end.
-
-  Fixpoint is_refl (r : PR Rbase) : bool :=
-    match r with
-      | PRinj _ => true
-      | _ => false
-    end.
-
-  Definition properAt (f : expr sym) (r : PR Rbase) : option (R Rbase) :=
-    if is_refl r then
-      to_R r
-    else
-      let results :=
-          match f with
-            | Inj And => (Rfunctorial (Rinj Eq) (Rfunctorial (Rinj Eq) (Rinj Eq)) ::
-                                      Rfunctorial (Rinj Impl) (Rfunctorial (Rinj Impl) (Rinj Impl)) :: nil)
-            | _ => nil
-          end
-      in
-      match filter (fun x => unify x r) results with
-        | nil => None
-        | r :: _ => Some r
-      end.
-
-  Definition atomic (tus : tenv typ) (e : expr sym) :
-    (forall e', TransitiveClosure.rightTrans (@expr_acc sym) e' e -> tenv typ -> PR Rbase -> option (T * R Rbase))
-    -> tenv typ -> R Rbase -> T :=
-    fun _ _ _ => e.
-
-  Definition app : T -> T -> R Rbase -> R Rbase -> T :=
-    fun a b _ _ => App a b.
-
-  Definition TR (us vs : env (typD ts)) (r : R Rbase) (t : T) (v : typD ts nil (typeForR typeForRbase r)) : Prop :=
-    exists v',
-      exprD us vs t (typeForR typeForRbase r) = Some v' /\
-      RD r v v'.
-
-  Theorem Hatomic
-  : forall e r r',
-      properAt e r = Some r' ->
-      instantiates typeForRbase r' r /\
-      forall us vs x result,
-        @atomic (typeof_env us) e (fun e _ => setoid_rewrite _ properAt atomic app (typeof_env us) e) (typeof_env vs) r' = result ->
-        exprD us vs e (typeForR typeForRbase r') = Some x ->
-        TR us vs r' result x.
-  Proof.
-    unfold TR, atomic, properAt; intros; subst.
-    split.
-    { admit. }
-    { intros; subst.
-      rewrite H1. eexists; split; eauto.
-      destruct result; simpl in *; try congruence.
-      admit. admit.  admit. admit. admit. }
-(*
-      destruct s; simpl in *; try congruence.
-      destruct r; try congruence.
-      { inv_all; subst. simpl.
-        intros; subst; auto. }
-      { red_exprD. simpl in *.
-        destruct r1; simpl in *; subst.
-        { destruct r; simpl in *; try congruence.
-          destruct r2; try congruence. inv_all. subst; simpl; intuition.
-          simpl in *. inv_all.
-          admit.
-          admit. admit. } admit. admit. } }
-*)
-  Qed.
-
-  Theorem Happ
-  : forall us vs t1 t2 r1 r2 v1 v2 f,
-      exprD us vs f (typeForR typeForRbase (Rfunctorial t1 t2)) = Some v1 ->
-      @TR us vs (Rfunctorial t1 t2) r1 v1 ->
-      @TR us vs t1 r2 v2 ->
-      @TR us vs t2 (app r1 r2 t1 t2) (v1 v2).
-  Proof.
-    unfold TR; simpl; intuition.
-    destruct H0. destruct H1. intuition.
-    unfold app. red_exprD.
-    cutrewrite (typeof_expr (typeof_env us) (typeof_env vs) r1 =
-                Some (tyArr (typeForR typeForRbase t1) (typeForR typeForRbase t2))).
-    { Cases.rewrite_all.
-      rewrite typ_cast_typ_refl. eexists; split; eauto. }
-    { admit. }
-  Qed.
-
-  Eval compute in
-      @setoid_rewrite _ _ _ _ _ properAt atomic app nil (Inj And) (tyProp :: nil)
-                      (PRfunctorial (PRguess _ tyProp) (PRfunctorial (PRguess _ tyProp) (PRinj Impl))).
-
-  Eval compute in typeof_expr nil (tyProp :: nil) (App (Inj And) (Var 0)).
-
-  Eval compute in
-      @setoid_rewrite _ _ _ _ _ properAt atomic app nil (Var 0) (tyProp :: nil)
-                      (PRinj Impl).
-
-  Eval compute in
-      @setoid_rewrite _ _ _ _ _ properAt atomic app nil (App (Inj And) (Var 0)) (tyProp :: nil)
-                      (PRfunctorial (PRguess _ tyProp) (PRinj Impl)).
-
-  Eval compute in
-      @setoid_rewrite _ _ _ _ _ properAt atomic app nil (App (App (Inj And) (Var 0)) (Var 0)) (tyProp :: nil)
-                      (PRinj Eq).
-End demo.
-**)
